theories/FV.v
@@ -1,5 +1,6 @@
+From LambdaST Require Import
+  Sets.
 From Coq Require Import
-  List
   String.
 
-Class FV (T : Type) := { fv : T -> list (* TODO: set *) string }.
+Class FV (T : Type) := { fv : T -> set string }.
