theories/Context.v
@@ -1,5 +1,6 @@
 From QuickChick Require Import QuickChick.
 From LambdaST Require Import
+  Sets
   FV
   Terms
   Types.
@@ -17,11 +18,11 @@ Hint Constructors context : core.
 Derive Show for context.
 Derive Arbitrary for context.
 
-Fixpoint fv_ctx ctx : list string :=
+Fixpoint fv_ctx ctx : set string :=
   match ctx with
-  | CtxEmpty => nil
-  | CtxHasTy x _ => cons x nil
-  | CtxComma lhs rhs | CtxSemic lhs rhs => fv_ctx lhs ++ fv_ctx rhs
+  | CtxEmpty => empty_set
+  | CtxHasTy x _ => singleton_set x
+  | CtxComma lhs rhs | CtxSemic lhs rhs => set_union (fv_ctx lhs) (fv_ctx rhs)
   end.
 
 Instance fv_context : FV context := { fv := fv_ctx; }.
